<?xml version="1.0" encoding="iso-8859-1"?>
<!DOCTYPE rdf:RDF [
	<!ENTITY rdf 'http://www.w3.org/1999/02/22-rdf-syntax-ns#'>
	<!ENTITY rdfs 'http://www.w3.org/2000/01/rdf-schema#'>
	<!ENTITY owl 'http://www.w3.org/2002/07/owl#'>
	<!ENTITY label 'http://purl.org/net/vocab/2004/03/label#'>
	<!ENTITY vann 'http://purl.org/vocab/vann/'>
	<!ENTITY cc 'http://web.resource.org/cc/'>
	<!ENTITY foaf 'http://xmlns.com/foaf/0.1/'>
	<!ENTITY dc 'http://purl.org/dc/elements/1.1/'>
	<!ENTITY dcterms 'http://purl.org/dc/terms/'>
]>
<rdf:RDF
	xml:lang="en"
	xml:base="&label;"
	xmlns:dcterms="&dcterms;"
	xmlns:dc="&dc;"
	xmlns:foaf="&foaf;"
	xmlns:cc="&cc;"
	xmlns:vann="&vann;"
	xmlns:label="&label;"
	xmlns:owl="&owl;"
	xmlns:rdfs="&rdfs;"
	xmlns:rdf="&rdf;">

<owl:Ontology rdf:about="">
	<rdfs:label>label</rdfs:label>
	<rdfs:comment>Term definitions for singular and plural label properties, and their inverses, for RDF terms</rdfs:comment>
	<rdfs:comment xml:lang="da">Definitioner for relationer mellem en term, dens inverse, og dens navn i entals- og flertalsform</rdfs:comment>
	<rdfs:comment xml:lang="es">Definiciones de etiquetas plurales y singulares de t&#233;rminos RDF</rdfs:comment>
	<owl:imports rdf:resource="http://www.w3.org/2000/01/rdf-schema"/>
	<owl:imports rdf:resource="http://www.w3.org/2002/07/owl"/>
	<foaf:maker>
		<foaf:Person>
			<foaf:name xml:lang="">Morten Høybye Frederiksen</foaf:name>
			<foaf:mbox_sha1sum xml:lang="">65b983bb397fb71849da910996741752ace8369b</foaf:mbox_sha1sum>
			<foaf:homepage rdf:resource="http://www.wasab.dk/morten/"/>
		</foaf:Person>
	</foaf:maker>
	<dcterms:created>2004-03-28</dcterms:created>
	<rdf:type rdf:resource="&cc;Work"/>
	<cc:license rdf:resource="http://creativecommons.org/licenses/by/1.0/"/>
</owl:Ontology>

<owl:AnnotationProperty rdf:ID="singular">
	<rdfs:label>singular</rdfs:label>
	<label:singular>singular form</label:singular>
	<label:plural>singular forms</label:plural>
	<rdfs:comment>A relation between a term and its label in literal singular form</rdfs:comment>
	<rdfs:label xml:lang="da">ental</rdfs:label>
	<label:singular xml:lang="da">entalsform</label:singular>
	<label:plural xml:lang="da">entalsformer</label:plural>
	<rdfs:comment xml:lang="da">En relation mellem en term og dens navn i entalsform</rdfs:comment>
	<rdfs:label xml:lang="es">singular</rdfs:label>
	<label:singular xml:lang="es">forma singular</label:singular>
	<label:plural xml:lang="es">formas singulares</label:plural>
	<rdfs:comment xml:lang="es">Una relaci&#243;n entre un t&#233;rmino y su etiqueta en forma singular</rdfs:comment>
	<rdfs:subPropertyOf rdf:resource="&rdfs;label"/>
	<rdfs:isDefinedBy rdf:resource=""/>
</owl:AnnotationProperty>

<owl:AnnotationProperty rdf:ID="plural">
	<rdfs:label>plural</rdfs:label>
	<label:singular>plural form</label:singular>
	<label:plural>plural forms</label:plural>
	<rdfs:comment>A relation between a term and its label in literal plural form</rdfs:comment>
	<rdfs:label xml:lang="da">flertal</rdfs:label>
	<label:singular xml:lang="da">flertalsform</label:singular>
	<label:plural xml:lang="da">flertalsformer</label:plural>
	<rdfs:comment xml:lang="da">En relation mellem en term og dens navn i flertalsform</rdfs:comment>
	<rdfs:label xml:lang="es">plural</rdfs:label>
	<label:singular xml:lang="es">forma plural</label:singular>
	<label:plural xml:lang="es">formas plurales</label:plural>
	<rdfs:comment xml:lang="es">Una relaci&#243;n entre un t&#233;rmino y su etiqueta en forma plural</rdfs:comment>
	<rdfs:subPropertyOf rdf:resource="&rdfs;label"/>
	<rdfs:isDefinedBy rdf:resource=""/>
	<vann:example><![CDATA[

]]></vann:example>
</owl:AnnotationProperty>

<owl:AnnotationProperty rdf:ID="inverseSingular">
	<rdfs:label>inverse singular</rdfs:label>
	<label:singular>singular form of inverse</label:singular>
	<label:plural>singular forms of inverses</label:plural>
	<rdfs:comment>A relation between a term and the label of its inverse in literal singular form</rdfs:comment>
	<rdfs:label xml:lang="da">inverst ental</rdfs:label>
	<label:singular xml:lang="da">entalsform for invers</label:singular>
	<label:plural xml:lang="da">entalsformer for inverse</label:plural>
	<rdfs:comment xml:lang="da">En relation mellem en term og dens inverses navn i entalsform</rdfs:comment>
	<rdfs:subPropertyOf rdf:resource="&rdfs;label"/>
	<rdfs:isDefinedBy rdf:resource=""/>
</owl:AnnotationProperty>

<owl:AnnotationProperty rdf:ID="inversePlural">
	<rdfs:label>inverse plural</rdfs:label>
	<label:singular>plural form of inverse</label:singular>
	<label:plural>plural forms of inverses</label:plural>
	<rdfs:comment>A relation between a term and the label of its inverse in literal plural form</rdfs:comment>
	<rdfs:label xml:lang="da">inverst flertal</rdfs:label>
	<label:singular xml:lang="da">flertalsform for invers</label:singular>
	<label:plural xml:lang="da">flertalsformer for inverse</label:plural>
	<rdfs:comment xml:lang="da">En relation mellem en term og dens inverses navn i flertalsform</rdfs:comment>
	<rdfs:subPropertyOf rdf:resource="&rdfs;label"/>
	<rdfs:isDefinedBy rdf:resource=""/>
</owl:AnnotationProperty>

</rdf:RDF>
